Fix the big-step small-step equivalence proof

metatheory/bigSmallEquivScript.sml
@@ -7,23 +7,23 @@ val _ = new_theory "bigSmallEquiv";
 (* ------------------------ Big step/small step equivalence ----------------- *)
 
 val small_eval_prefix = Q.prove (
-`∀cenv env e c cenv' env' e' c' r.
-  e_step_reln^* (cenv,env,Exp e,c) (cenv,env',Exp e',c') ∧
-  small_eval cenv env' e' c' r
+`∀cenv s env e c cenv' s' env' e' c' r.
+  e_step_reln^* (cenv,s,env,Exp e,c) (cenv,s',env',Exp e',c') ∧
+  small_eval cenv s' env' e' c' r
   ⇒
-  small_eval cenv env e c r`,
+  small_eval cenv s env e c r`,
 rw [] >>
 cases_on `r` >|
-[all_tac,
+[cases_on `a`,
  cases_on `e''`] >>
 fs [small_eval_def] >>
 metis_tac [transitive_RTC, transitive_def]);
 
 val e_single_step_add_ctxt = Q.prove (
-`!cenv env e c cenv' env' e' c' c''.
-  (e_step (cenv,env,e,c) = Estep (cenv',env',e',c'))
+`!cenv s env e c cenv' s' env' e' c' c''.
+  (e_step (cenv,s,env,e,c) = Estep (cenv',s',env',e',c'))
   ⇒
-  (e_step (cenv,env,e,c++c'') = Estep (cenv',env',e',c'++c''))`,
+  (e_step (cenv,s,env,e,c++c'') = Estep (cenv',s',env',e',c'++c''))`,
 rw [e_step_def] >>
 cases_on `e` >>
 fs [push_def, return_def, emp_def] >>
@@ -45,10 +45,10 @@ fs [push_def, return_def] >>
 rw []);
 
 val e_single_error_add_ctxt = Q.prove (
-`!cenv env e c cenv' env' e' c' c''.
-  (e_step (cenv,env,e,c) = Etype_error)
+`!cenv s env e c c'.
+  (e_step (cenv,s,env,e,c) = Etype_error)
   ⇒
-  (e_step (cenv,env,e,c++c'') = Etype_error)`,
+  (e_step (cenv,s,env,e,c++c') = Etype_error)`,
 rw [e_step_def] >>
 cases_on `e` >>
 fs [push_def, return_def, emp_def] >>
@@ -71,16 +71,14 @@ rw []);
 
 val e_step_add_ctxt_help = Q.prove (
 `!st1 st2. e_step_reln^* st1 st2 ⇒
-  !cenv1 env1 e1 c1 cenv2 env2 e2 c2 c'.
-    (st1 = (cenv1,env1,e1,c1)) ∧ (st2 = (cenv2,env2,e2,c2))
+  !cenv1 s1 env1 e1 c1 cenv2 s2 env2 e2 c2 c'.
+    (st1 = (cenv1,s1,env1,e1,c1)) ∧ (st2 = (cenv2,s2,env2,e2,c2))
     ⇒
-    e_step_reln^* (cenv1,env1,e1,c1++c') (cenv2,env2,e2,c2++c')`,
+    e_step_reln^* (cenv1,s1,env1,e1,c1++c') (cenv2,s2,env2,e2,c2++c')`,
 HO_MATCH_MP_TAC RTC_INDUCT >>
 rw [e_step_reln_def] >-
 metis_tac [RTC_REFL] >>
-cases_on `st1'` >>
-cases_on `r` >>
-cases_on `r'` >>
+PairCases_on `st1'` >>
 fs [] >>
 imp_res_tac e_single_step_add_ctxt >>
 fs [] >>
@@ -88,30 +86,30 @@ rw [Once RTC_CASES1] >>
 metis_tac [e_step_reln_def]);
 
 val e_step_add_ctxt = Q.prove (
-`!cenv1 env1 e1 c1 cenv2 env2 e2 c2 c'.
-   e_step_reln^* (cenv1,env1,e1,c1) (cenv2,env2,e2,c2)
+`!cenv1 s1 env1 e1 c1 cenv2 s2 env2 e2 c2 c'.
+   e_step_reln^* (cenv1,s1,env1,e1,c1) (cenv2,s2,env2,e2,c2)
    ⇒
-   e_step_reln^* (cenv1,env1,e1,c1++c') (cenv2,env2,e2,c2++c')`,
+   e_step_reln^* (cenv1,s1,env1,e1,c1++c') (cenv2,s2,env2,e2,c2++c')`,
 metis_tac [e_step_add_ctxt_help]);
 
 val e_step_raise = Q.prove (
-`!cenv env err c.
-  e_step_reln^* (cenv,env,Exp (Raise err),c) (cenv,env,Exp (Raise err),[])`,
+`!cenv s env err c.
+  e_step_reln^* (cenv,s,env,Exp (Raise err),c) (cenv,s,env,Exp (Raise err),[])`,
 induct_on `c` >>
 rw [] >>
 rw [Once RTC_CASES1] >>
-qexists_tac `(cenv,env,Exp (Raise err),c)` >>
+qexists_tac `(cenv,s,env,Exp (Raise err),c)` >>
 rw [e_step_reln_def, e_step_def]);
 
 val small_eval_err_add_ctxt = Q.prove (
-`!cenv env e c err c'.
- small_eval cenv env e c (Rerr err) ⇒ small_eval cenv env e (c++c') (Rerr err)`,
+`!cenv s env e c err c'.
+ small_eval cenv s env e c (Rerr err) ⇒ small_eval cenv s env e (c++c') (Rerr err)`,
 cases_on `err` >>
 rw [small_eval_def] >|
-[`e_step_reln^* (cenv,env,Exp e,c++c') (cenv,env',e',c''++c')`
+[`e_step_reln^* (cenv,s,env,Exp e,c++c') (cenv,s',env',e',c''++c')`
        by metis_tac [e_step_add_ctxt] >>
      metis_tac [e_single_error_add_ctxt],
- `e_step_reln^* (cenv,env,Exp e',c++c') (cenv,env',Exp (Raise e),c')`
+ `e_step_reln^* (cenv,s,env,Exp e',c++c') (cenv,s',env',Exp (Raise e),c')`
        by metis_tac [e_step_add_ctxt, APPEND] >>
      metis_tac [e_step_raise, transitive_RTC, transitive_def]]);
 
@@ -120,7 +118,7 @@ rw [do_con_check_def] >>
 every_case_tac >>
 fs [] >>
 cases_on `r` >|
-[all_tac,
+[cases_on `a`,
  cases_on `e`] >>
 rw [small_eval_def] >>
 EQ_TAC >>
@@ -158,280 +156,296 @@ rw [] >|
      metis_tac []];
 
 val small_eval_con = Q.prove (
-`!cenv env cn e1 es ns c r.
+`!cenv s env cn e1 es ns c r.
   do_con_check cenv cn (LENGTH (e1::es))
   ⇒
-  (small_eval cenv env (Con cn (e1::es)) c r =
-   small_eval cenv env e1 ((Ccon cn [] () es,env)::c) r)`,
+  (small_eval cenv s env (Con cn (e1::es)) c r =
+   small_eval cenv s env e1 ((Ccon cn [] () es,env)::c) r)`,
 rw [do_con_check_def] >>
 every_case_tac >>
 fs [] >>
 small_eval_step_tac);
 
 val small_eval_app = Q.prove (
-`!cenv env op e1 e2 c r.
-  small_eval cenv env (App op e1 e2) c r =
-  small_eval cenv env e1 ((Capp1 op () e2,env)::c) r`,
+`!cenv s env op e1 e2 c r.
+  small_eval cenv s env (App op e1 e2) c r =
+  small_eval cenv s env e1 ((Capp1 op () e2,env)::c) r`,
+small_eval_step_tac);
+
+val small_eval_uapp = Q.prove (
+`!cenv s env uop e1 c r.
+  small_eval cenv s env (Uapp uop e1) c r =
+  small_eval cenv s env e1 ((Cuapp uop (),env)::c) r`,
 small_eval_step_tac);
 
 val small_eval_log = Q.prove (
-`!cenv env op e1 e2 c r.
-  small_eval cenv env (Log op e1 e2) c r =
-  small_eval cenv env e1 ((Clog op () e2,env)::c) r`,
+`!cenv s env op e1 e2 c r.
+  small_eval cenv s env (Log op e1 e2) c r =
+  small_eval cenv s env e1 ((Clog op () e2,env)::c) r`,
 small_eval_step_tac);
 
 val small_eval_if = Q.prove (
-`!cenv env e1 e2 e3 c r.
-  small_eval cenv env (If e1 e2 e3) c r =
-  small_eval cenv env e1 ((Cif () e2 e3,env)::c) r`,
+`!cenv s env e1 e2 e3 c r.
+  small_eval cenv s env (If e1 e2 e3) c r =
+  small_eval cenv s env e1 ((Cif () e2 e3,env)::c) r`,
 small_eval_step_tac);
 
 val small_eval_match = Q.prove (
-`!cenv env e1 pes c r.
-  small_eval cenv env (Mat e1 pes) c r =
-  small_eval cenv env e1 ((Cmat () pes,env)::c) r`,
+`!cenv s env e1 pes c r.
+  small_eval cenv s env (Mat e1 pes) c r =
+  small_eval cenv s env e1 ((Cmat () pes,env)::c) r`,
 small_eval_step_tac);
 
 val small_eval_let = Q.prove (
-`!cenv env n e1 e2 c r.
-  small_eval cenv env (Let n e1 e2) c r =
-  small_eval cenv env e1 ((Clet n () e2,env)::c) r`,
+`!cenv s env n e1 e2 c r.
+  small_eval cenv s env (Let n e1 e2) c r =
+  small_eval cenv s env e1 ((Clet n () e2,env)::c) r`,
 small_eval_step_tac);
 
 val small_eval_letrec = Q.prove (
-`!cenv env funs e1 c r.
+`!cenv s env funs e1 c r.
   ALL_DISTINCT (MAP (λ(x,y,z). x) funs) ⇒
-  (small_eval cenv env (Letrec funs e1) c r =
-   small_eval cenv (build_rec_env funs env) e1 c r)`,
+  (small_eval cenv s env (Letrec funs e1) c r =
+   small_eval cenv s (build_rec_env funs env) e1 c r)`,
 small_eval_step_tac);
 
 val (small_eval_list_rules, small_eval_list_ind, small_eval_list_cases) = Hol_reln `
-(!cenv env. small_eval_list cenv env [] (Rval [])) ∧
-(!cenv env e es v vs env'.
-  e_step_reln^* (cenv,env,Exp e,[]) (cenv,env',Val v,[]) ∧
-  small_eval_list cenv env es (Rval vs)
+(!cenv s env. small_eval_list cenv s env [] (Rval (s,[]))) ∧
+(!cenv s1 env e es v vs s2 s3 env'.
+  e_step_reln^* (cenv,s1,env,Exp e,[]) (cenv,s2,env',Val v,[]) ∧
+  small_eval_list cenv s2 env es (Rval (s3,vs))
   ⇒
-  small_eval_list cenv env (e::es) (Rval (v::vs))) ∧
-(!cenv env e es err env' v.
-  e_step_reln^* (cenv,env,Exp e,[]) (cenv,env',Exp (Raise err),[]) ∨
-  (e_step_reln^* (cenv,env,Exp e,[]) (cenv,env',Val v,[]) ∧
-   small_eval_list cenv env es (Rerr (Rraise err)))
+  small_eval_list cenv s1 env (e::es) (Rval (s3,v::vs))) ∧
+(!cenv s1 env e es err env' s2 v.
+  e_step_reln^* (cenv,s1,env,Exp e,[]) (cenv,s2,env',Exp (Raise err),[]) ∨
+  (e_step_reln^* (cenv,s1,env,Exp e,[]) (cenv,s2,env',Val v,[]) ∧
+   small_eval_list cenv s2 env es (Rerr (Rraise err)))
   ⇒
-  (small_eval_list cenv env (e::es) (Rerr (Rraise err)))) ∧
-(!cenv env e es e' c' env' v.
-  (e_step_reln^* (cenv,env,Exp e,[]) (cenv,env',e',c') ∧
-   (e_step (cenv,env',e',c') = Etype_error)) ∨
-  (e_step_reln^* (cenv,env,Exp e,[]) (cenv,env',Val v,[]) ∧
-   small_eval_list cenv env es (Rerr Rtype_error))
+  (small_eval_list cenv s1 env (e::es) (Rerr (Rraise err)))) ∧
+(!cenv s1 env e es e' c' env' s2 v.
+  (e_step_reln^* (cenv,s1,env,Exp e,[]) (cenv,s2,env',e',c') ∧
+   (e_step (cenv,s2,env',e',c') = Etype_error)) ∨
+  (e_step_reln^* (cenv,s1,env,Exp e,[]) (cenv,s2,env',Val v,[]) ∧
+   small_eval_list cenv s2 env es (Rerr Rtype_error))
   ⇒
-  (small_eval_list cenv env (e::es) (Rerr Rtype_error)))`;
+  (small_eval_list cenv s1 env (e::es) (Rerr Rtype_error)))`;
 
 val small_eval_list_length = Q.prove (
-`!cenv env es r. small_eval_list cenv env es r ⇒
-  !vs. (r = Rval vs) ⇒ (LENGTH es = LENGTH vs)`,
+`!cenv s1 env es r. small_eval_list cenv s1 env es r ⇒
+  !vs s2. (r = Rval (s2,vs)) ⇒ (LENGTH es = LENGTH vs)`,
 HO_MATCH_MP_TAC small_eval_list_ind >>
 rw [] >>
 rw []);
 
 val small_eval_list_step = Q.prove (
-`!cenv env es r. small_eval_list cenv env es r ⇒
-  (!e v vs cn vs' env'.
+`!cenv s2 env es r. small_eval_list cenv s2 env es r ⇒
+  (!e v vs cn vs' env' s1 s3.
      do_con_check cenv cn (LENGTH vs' + 1 + LENGTH vs) ∧
-     (r = Rval vs) ∧ e_step_reln^* (cenv,env,Exp e,[]) (cenv,env',Val v,[]) ⇒
-     e_step_reln^* (cenv,env,Exp e,[(Ccon cn vs' () es,env)])
-                   (cenv,env,Val (Conv cn (REVERSE vs'++[v]++vs)),[]))`,
+     (r = Rval (s3,vs)) ∧ e_step_reln^* (cenv,s1,env,Exp e,[]) (cenv,s2,env',Val v,[]) ⇒
+     e_step_reln^* (cenv,s1,env,Exp e,[(Ccon cn vs' () es,env)])
+                   (cenv,s3,env,Val (Conv cn (REVERSE vs'++[v]++vs)),[]))`,
 HO_MATCH_MP_TAC (fetch "-" "small_eval_list_strongind") >>
 rw [] >|
-[`e_step_reln^* (cenv,env,Exp e,[(Ccon cn vs' () [],env)])
-                (cenv,env',Val v,[(Ccon cn vs' () [],env)])`
+[`e_step_reln^* (cenv,s1,env,Exp e,[(Ccon cn vs' () [],env)])
+                (cenv,s2,env',Val v,[(Ccon cn vs' () [],env)])`
              by metis_tac [e_step_add_ctxt,APPEND] >>
-     `e_step_reln (cenv,env',Val v,[(Ccon cn vs' () [],env)])
-                  (cenv,env,Val (Conv cn (REVERSE vs' ++ [v] ++ [])),[])`
+     `e_step_reln (cenv,s2,env',Val v,[(Ccon cn vs' () [],env)])
+                  (cenv,s2,env,Val (Conv cn (REVERSE vs' ++ [v] ++ [])),[])`
              by rw [return_def, continue_def, e_step_reln_def, e_step_def] >>
      fs [] >>
      metis_tac [transitive_RTC, transitive_def, RTC_SINGLE, APPEND],
  `LENGTH (v'::vs'') + 1 + LENGTH vs = LENGTH vs'' + 1 + SUC (LENGTH vs)`
               by (fs [] >>
                   DECIDE_TAC) >>
-     `e_step_reln^* (cenv,env,Exp e,[(Ccon cn (v'::vs'') () es,env)])
-                (cenv,env,Val (Conv cn (REVERSE vs'' ++ [v'] ++ [v] ++ vs)),[])`
+     `e_step_reln^* (cenv,s2,env,Exp e,[(Ccon cn (v'::vs'') () es,env)])
+                (cenv,s3,env,Val (Conv cn (REVERSE vs'' ++ [v'] ++ [v] ++ vs)),[])`
              by metis_tac [REVERSE_DEF] >>
-     `e_step_reln^* (cenv,env,Exp e',[(Ccon cn vs'' () (e::es),env)])
-                    (cenv,env'',Val v',[(Ccon cn vs'' () (e::es),env)])`
+     `e_step_reln^* (cenv,s1,env,Exp e',[(Ccon cn vs'' () (e::es),env)])
+                    (cenv,s2,env'',Val v',[(Ccon cn vs'' () (e::es),env)])`
              by metis_tac [e_step_add_ctxt, APPEND] >>
-     `e_step_reln (cenv,env'',Val v',[(Ccon cn vs'' () (e::es),env)])
-                  (cenv,env,Exp e,[(Ccon cn (v'::vs'') () es,env)])`
+     `e_step_reln (cenv,s2,env'',Val v',[(Ccon cn vs'' () (e::es),env)])
+                  (cenv,s2,env,Exp e,[(Ccon cn (v'::vs'') () es,env)])`
              by rw [push_def,continue_def, e_step_reln_def, e_step_def] >>
      fs [] >>
      `LENGTH es = LENGTH vs` by metis_tac [small_eval_list_length] >>
      `LENGTH vs'' + 1 + 1 + LENGTH es = LENGTH vs'' + 1 + SUC (LENGTH es)`
                 by DECIDE_TAC >>
-     `e_step_reln^* (cenv,env,Exp e',[(Ccon cn vs'' () (e::es),env)])
-                    (cenv,env,Val (Conv cn (REVERSE vs'' ++ [v'] ++ [v] ++ vs)),[])`
+     `e_step_reln^* (cenv,s1,env,Exp e',[(Ccon cn vs'' () (e::es),env)])
+                    (cenv,s3,env,Val (Conv cn (REVERSE vs'' ++ [v'] ++ [v] ++ vs)),[])`
                 by metis_tac [RTC_SINGLE, transitive_RTC, transitive_def] >>
      metis_tac [APPEND_ASSOC, APPEND]]);
 
 val small_eval_list_err = Q.prove (
-`!cenv env es r. small_eval_list cenv env es r ⇒
-  (!e v err cn vs' env'.
+`!cenv s2 env es r. small_eval_list cenv s2 env es r ⇒
+  (!e v err cn vs' env' s1.
      do_con_check cenv cn (LENGTH vs' + 1 + LENGTH es) ∧
      (r = Rerr (Rraise err)) ∧
-     e_step_reln^* (cenv,env,e,[]) (cenv,env',Val v,[]) ⇒
-     ?env''. e_step_reln^* (cenv,env,e,[(Ccon cn vs' () es,env)])
-                           (cenv,env'',Exp (Raise err),[]))`,
+     e_step_reln^* (cenv,s1,env,e,[]) (cenv,s2,env',Val v,[]) ⇒
+     ?s3 env''. e_step_reln^* (cenv,s1,env,e,[(Ccon cn vs' () es,env)])
+                              (cenv,s3,env'',Exp (Raise err),[]))`,
 HO_MATCH_MP_TAC small_eval_list_ind >>
 rw [] >>
-`e_step_reln^* (cenv,env,e',[(Ccon cn vs' () (e::es),env)])
-               (cenv,env'',Val v',[(Ccon cn vs' () (e::es),env)])`
+`e_step_reln^* (cenv,s1,env,e',[(Ccon cn vs' () (e::es),env)])
+               (cenv,s2,env'',Val v',[(Ccon cn vs' () (e::es),env)])`
              by metis_tac [e_step_add_ctxt, APPEND] >>
-`e_step_reln (cenv,env'',Val v',[(Ccon cn vs' () (e::es),env)])
-             (cenv,env,Exp e,[(Ccon cn (v'::vs') () es,env)])`
+`e_step_reln (cenv,s2,env'',Val v',[(Ccon cn vs' () (e::es),env)])
+             (cenv,s2,env,Exp e,[(Ccon cn (v'::vs') () es,env)])`
         by rw [push_def,continue_def, e_step_reln_def, e_step_def] >>
 `LENGTH vs' + 1 + 1 + LENGTH es = LENGTH vs' + 1 + SUC (LENGTH es)`
                 by DECIDE_TAC >>
 fs [] >|
-[`e_step_reln^* (cenv,env,Exp e,[(Ccon cn (v'::vs') () es,env)])
-                (cenv,env',Exp (Raise err),[(Ccon cn (v'::vs') () es,env)])`
+[`e_step_reln^* (cenv,s2,env,Exp e,[(Ccon cn (v'::vs') () es,env)])
+                (cenv,s2',env',Exp (Raise err),[(Ccon cn (v'::vs') () es,env)])`
              by metis_tac [e_step_add_ctxt,APPEND] >>
-     `e_step_reln^* (cenv,env',Exp (Raise err),[(Ccon cn (v'::vs') () es,env)])
-                    (cenv,env',Exp (Raise err),[])`
+     `e_step_reln^* (cenv,s2',env',Exp (Raise err),[(Ccon cn (v'::vs') () es,env)])
+                    (cenv,s2',env',Exp (Raise err),[])`
              by metis_tac [e_step_raise] >>
      metis_tac [RTC_SINGLE, transitive_RTC, transitive_def],
  `LENGTH (v'::vs') + 1 + LENGTH es = LENGTH vs' + 1 + SUC (LENGTH es)`
               by (fs [] >>
                   DECIDE_TAC) >>
-     `?env''. e_step_reln^* (cenv,env,Exp e,[(Ccon cn (v'::vs') () es,env)])
-                        (cenv,env'',Exp (Raise err), [])`
+     `?s3 env''. e_step_reln^* (cenv,s2,env,Exp e,[(Ccon cn (v'::vs') () es,env)])
+                               (cenv,s3,env'',Exp (Raise err), [])`
              by metis_tac [] >>
      metis_tac [RTC_SINGLE, transitive_RTC, transitive_def]]);
 
 val small_eval_list_terr = Q.prove (
-`!cenv env es r. small_eval_list cenv env es r ⇒
-  (!e v err cn vs' env'.
+`!cenv s2 env es r. small_eval_list cenv s2 env es r ⇒
+  (!e v err cn vs' env' s1.
      do_con_check cenv cn (LENGTH vs' + 1 + LENGTH es) ∧
      (r = Rerr Rtype_error) ∧
-     e_step_reln^* (cenv,env,e,[]) (cenv,env',Val v,[]) ⇒
-     ?env'' e' c'. e_step_reln^* (cenv,env,e,[(Ccon cn vs' () es,env)])
-                                 (cenv,env'',e',c') ∧
-                   (e_step (cenv,env'',e',c') = Etype_error))`,
+     e_step_reln^* (cenv,s1,env,e,[]) (cenv,s2,env',Val v,[]) ⇒
+     ?s3 env'' e' c'. e_step_reln^* (cenv,s1,env,e,[(Ccon cn vs' () es,env)])
+                                    (cenv,s3,env'',e',c') ∧
+                   (e_step (cenv,s3,env'',e',c') = Etype_error))`,
 HO_MATCH_MP_TAC small_eval_list_ind >>
 rw [] >>
-`e_step_reln^* (cenv,env,e'',[(Ccon cn vs' () (e::es),env)])
-               (cenv,env'',Val v',[(Ccon cn vs' () (e::es),env)])`
+`e_step_reln^* (cenv,s1,env,e'',[(Ccon cn vs' () (e::es),env)])
+               (cenv,s2,env'',Val v',[(Ccon cn vs' () (e::es),env)])`
              by metis_tac [e_step_add_ctxt, APPEND] >>
-`e_step_reln (cenv,env'',Val v',[(Ccon cn vs' () (e::es),env)])
-             (cenv,env,Exp e,[(Ccon cn (v'::vs') () es,env)])`
+`e_step_reln (cenv,s2,env'',Val v',[(Ccon cn vs' () (e::es),env)])
+             (cenv,s2,env,Exp e,[(Ccon cn (v'::vs') () es,env)])`
         by rw [push_def,continue_def, e_step_reln_def, e_step_def] >>
 `LENGTH vs' + 1 + 1 + LENGTH es = LENGTH vs' + 1 + SUC (LENGTH es)`
                 by DECIDE_TAC >>
 fs [] >|
-[`e_step_reln^* (cenv,env,Exp e,[(Ccon cn (v'::vs') () es,env)])
-                (cenv,env',e',c'++[(Ccon cn (v'::vs') () es,env)])`
+[`e_step_reln^* (cenv,s2,env,Exp e,[(Ccon cn (v'::vs') () es,env)])
+                (cenv,s2',env',e',c'++[(Ccon cn (v'::vs') () es,env)])`
              by metis_tac [e_step_add_ctxt,APPEND] >>
-     `e_step (cenv,env',e',c'++[(Ccon cn (v'::vs') () es,env)]) = Etype_error`
+     `e_step (cenv,s2',env',e',c'++[(Ccon cn (v'::vs') () es,env)]) = Etype_error`
              by metis_tac [e_single_error_add_ctxt] >>
      metis_tac [RTC_SINGLE, transitive_RTC, transitive_def],
  `LENGTH (v'::vs') + 1 + LENGTH es = LENGTH vs' + 1 + SUC (LENGTH es)`
               by (fs [] >>
                   DECIDE_TAC) >>
-     `?env'' e' c'. e_step_reln^* (cenv,env,Exp e,[(Ccon cn (v'::vs') () es,env)])
-                              (cenv,env'',e',c') ∧
-                (e_step (cenv,env'',e',c') = Etype_error)`
+     `?s'' env'' e' c'. e_step_reln^* (cenv,s2,env,Exp e,[(Ccon cn (v'::vs') () es,env)])
+                              (cenv,s'',env'',e',c') ∧
+                (e_step (cenv,s'',env'',e',c') = Etype_error)`
              by metis_tac [] >>
      metis_tac [RTC_SINGLE, transitive_RTC, transitive_def]]);
 
 val (small_eval_match_rules, small_eval_match_ind, small_eval_match_cases) = Hol_reln `
-(!cenv env v. small_eval_match cenv env v [] (Rerr (Rraise Bind_error))) ∧
-(!cenv env p e pes r env' v.
+(!cenv s env v. small_eval_match cenv s env v [] (Rerr (Rraise Bind_error))) ∧
+(!cenv s env p e pes r env' v.
   ALL_DISTINCT (pat_bindings p []) ∧
-  (pmatch cenv p v env = Match env') ∧
-  small_eval cenv env' e [] r
+  (pmatch cenv s p v env = Match env') ∧
+  small_eval cenv s env' e [] r
   ⇒
-  small_eval_match cenv env v ((p,e)::pes) r) ∧
-(!cenv env e p pes r v.
+  small_eval_match cenv s env v ((p,e)::pes) r) ∧
+(!cenv s env e p pes r v.
   ALL_DISTINCT (pat_bindings p []) ∧
-  (pmatch cenv p v env = No_match) ∧
-  small_eval_match cenv env v pes r
+  (pmatch cenv s p v env = No_match) ∧
+  small_eval_match cenv s env v pes r
   ⇒
-  small_eval_match cenv env v ((p,e)::pes) r) ∧
-(!cenv env p e pes v.
+  small_eval_match cenv s env v ((p,e)::pes) r) ∧
+(!cenv s env p e pes v.
   ¬(ALL_DISTINCT (pat_bindings p []))
   ⇒
-  small_eval_match cenv env v ((p,e)::pes) (Rerr (Rtype_error))) ∧
-(!cenv env p e pes v.
-  (pmatch cenv p v env = Match_type_error)
+  small_eval_match cenv s env v ((p,e)::pes) (Rerr (Rtype_error))) ∧
+(!cenv s env p e pes v.
+  (pmatch cenv s p v env = Match_type_error)
   ⇒
-  small_eval_match cenv env v ((p,e)::pes) (Rerr (Rtype_error)))`;
+  small_eval_match cenv s env v ((p,e)::pes) (Rerr (Rtype_error)))`;
 
 val alt_small_eval_def = Define `
-(alt_small_eval cenv env e c (Rval v) =
-    ∃env'. e_step_reln^* (cenv,env,e,c) (cenv,env',Val v,[])) ∧
-(alt_small_eval cenv env e c (Rerr (Rraise err)) ⇔
-    ∃env'.
-      e_step_reln^* (cenv,env,e,c) (cenv,env',Exp (Raise err),[])) ∧
-(alt_small_eval cenv env e c (Rerr Rtype_error) ⇔
-    ∃env' e' c'.
-      e_step_reln^* (cenv,env,e,c) (cenv,env',e',c') ∧
-      (e_step (cenv,env',e',c') = Etype_error))`;
+(alt_small_eval cenv s1 env e c (Rval (s2,v)) =
+    ∃env'. e_step_reln^* (cenv,s1,env,e,c) (cenv,s2,env',Val v,[])) ∧
+(alt_small_eval cenv s1 env e c (Rerr (Rraise err)) ⇔
+    ∃s2 env'.
+      e_step_reln^* (cenv,s1,env,e,c) (cenv,s2,env',Exp (Raise err),[])) ∧
+(alt_small_eval cenv s env e c (Rerr Rtype_error) ⇔
+    ∃s2 env' e' c'.
+      e_step_reln^* (cenv,s1,env,e,c) (cenv,s2,env',e',c') ∧
+      (e_step (cenv,s2,env',e',c') = Etype_error))`;
 
 val small_eval_match_thm = Q.prove (
-`!cenv env v pes r. small_eval_match cenv env v pes r ⇒
- !env2. alt_small_eval cenv env2 (Val v) [(Cmat () pes,env)] r`,
+`!cenv s env v pes r. small_eval_match cenv s env v pes r ⇒
+ !env2. alt_small_eval cenv s env2 (Val v) [(Cmat () pes,env)] r`,
 HO_MATCH_MP_TAC small_eval_match_ind >>
 rw [alt_small_eval_def] >|
-[qexists_tac `env` >>
+[qexists_tac `s` >>
+     qexists_tac `env` >>
      match_mp_tac RTC_SINGLE >>
      rw [e_step_reln_def, e_step_def, continue_def],
  cases_on `r` >|
-     [all_tac,
+     [cases_on `a`,
       cases_on `e'`] >>
-     fs [alt_small_eval_def, small_eval_def] >>
-     qexists_tac `env''` >>
-     rw [Once RTC_CASES1, e_step_reln_def] >|
-     [rw [e_step_def, continue_def],
-      qexists_tac `e'` >>
+     fs [alt_small_eval_def, small_eval_def] >|
+     [qexists_tac `env''` >>
+          rw [Once RTC_CASES1, e_step_reln_def] >>
+          rw [e_step_def, continue_def],
+      qexists_tac `s'` >>
+          qexists_tac `env''` >>
+          rw [Once RTC_CASES1, e_step_reln_def] >>
+          qexists_tac `e'` >>
           qexists_tac `c'` >>
           rw [] >>
           rw [e_step_def, continue_def],
-      rw [e_step_def, continue_def]],
+      qexists_tac `s'` >>
+          qexists_tac `env''` >>
+          rw [Once RTC_CASES1, e_step_reln_def] >>
+          rw [e_step_def, continue_def]],
  cases_on `r` >|
-     [all_tac,
+     [cases_on `a`,
       cases_on `e'`] >>
      fs [alt_small_eval_def] >>
      rw [Once RTC_CASES1, e_step_reln_def] >|
      [rw [e_step_def, push_def, continue_def],
       pop_assum (ASSUME_TAC o Q.SPEC `env`) >>
           fs [] >>
+          qexists_tac `s2` >>
           qexists_tac `env'` >>
           qexists_tac `e'` >>
           qexists_tac `c'` >>
           rw [] >>
           rw [e_step_def, push_def, continue_def],
       rw [e_step_def, push_def, continue_def]],
- qexists_tac `env2` >>
+ qexists_tac `s` >>
+     qexists_tac `env2` >>
      qexists_tac `Val v` >>
      qexists_tac `[(Cmat () ((p,e)::pes),env)]` >>
      rw [RTC_REFL] >>
      rw [e_step_def, continue_def],
- qexists_tac `env2` >>
+ qexists_tac `s` >>
+     qexists_tac `env2` >>
      qexists_tac `Val v` >>
      qexists_tac `[(Cmat () ((p,e)::pes),env)]` >>
      rw [RTC_REFL] >>
      rw [e_step_def, continue_def]]);
 
 val big_exp_to_small_exp = Q.prove (
-`(∀ cenv env e r.
-   evaluate cenv env e r ⇒
-   small_eval cenv env e [] r) ∧
- (∀ cenv env es r.
-   evaluate_list cenv env es r ⇒
-   small_eval_list cenv env es r) ∧
- (∀ cenv env v pes r.
-   evaluate_match cenv env v pes r ⇒
-   small_eval_match cenv env v pes r)`,
+`(∀cenv s env e r.
+   evaluate cenv s env e r ⇒
+   small_eval cenv s env e [] r) ∧
+ (∀cenv s env es r.
+   evaluate_list cenv s env es r ⇒
+   small_eval_list cenv s env es r) ∧
+ (∀cenv s env v pes r.
+   evaluate_match cenv s env v pes r ⇒
+   small_eval_match cenv s env v pes r)`,
 HO_MATCH_MP_TAC evaluate_ind >>
 rw [small_eval_app, small_eval_log, small_eval_if, small_eval_match,
-    small_eval_let, small_eval_letrec] >|
+    small_eval_let, small_eval_letrec,small_eval_uapp] >|
 [rw [return_def, small_eval_def, Once RTC_CASES1, e_step_reln_def, e_step_def] >>
      metis_tac [RTC_REFL],
  rw [return_def, small_eval_def, Once RTC_CASES1, e_step_reln_def, e_step_def] >>
@@ -443,19 +457,20 @@ rw [small_eval_app, small_eval_log, small_eval_if, small_eval_match,
           fs [Once small_eval_list_cases] >>
           rw [return_def, small_eval_def, Once RTC_CASES1, e_step_reln_def, e_step_def] >>
           metis_tac [RTC_REFL],
-      fs [Once small_eval_list_cases]  >>
+      fs [Once small_eval_list_cases] >>
           rw [small_eval_def] >>
           `SUC (LENGTH t) = LENGTH ([]:v list) + 1 + LENGTH t` by
                   (fs [] >>
                    DECIDE_TAC) >>
           `do_con_check cenv cn (LENGTH ([]:v list) + 1 + LENGTH vs')`
                       by metis_tac [small_eval_list_length] >>
-          `e_step_reln^* (cenv,env,Exp h,[(Ccon cn [] () t,env)])
-                         (cenv,env,Val (Conv cn (REVERSE ([]:v list)++[v]++vs')),[])`
+          `e_step_reln^* (cenv,s,env,Exp h,[(Ccon cn [] () t,env)])
+                         (cenv,s',env,Val (Conv cn (REVERSE ([]:v list)++[v]++vs')),[])`
                     by metis_tac [small_eval_list_step] >>
           fs [] >>
           metis_tac []],
  rw [small_eval_def, e_step_def] >>
+     qexists_tac `s` >>
      qexists_tac `env` >>
      qexists_tac `Exp (Con cn es)` >>
      rw [] >>
@@ -480,6 +495,7 @@ rw [small_eval_app, small_eval_log, small_eval_if, small_eval_match,
      qexists_tac `env` >>
      rw [Once RTC_CASES1, e_step_reln_def, return_def, e_step_def],
  rw [small_eval_def, e_step_def] >>
+     qexists_tac `s` >>
      qexists_tac `env` >>
      qexists_tac `Exp (Var n)` >>
      rw [] >>
@@ -488,102 +504,122 @@ rw [small_eval_app, small_eval_log, small_eval_if, small_eval_match,
      qexists_tac `env` >>
      rw [Once RTC_CASES1, e_step_reln_def, return_def, e_step_def],
  fs [small_eval_def] >>
-     `e_step_reln^* (cenv,env,Exp e,[(Capp1 op () e',env)])
-                (cenv,env'',Val v1,[(Capp1 op () e',env)])`
+     `e_step_reln^* (cenv,s,env,Exp e,[(Cuapp uop (),env)])
+                    (cenv,s2,env',Val v,[(Cuapp uop (),env)])`
              by metis_tac [e_step_add_ctxt, APPEND] >>
-     `e_step_reln (cenv,env'',Val v1,[(Capp1 op () e',env)])
-                  (cenv,env,Exp e',[(Capp2 op v1 (),env)])`
-             by rw [e_step_def, e_step_reln_def, continue_def, push_def] >>
-     `e_step_reln^* (cenv,env,Exp e',[(Capp2 op v1 (),env)])
-                    (cenv,env''',Val v2,[(Capp2 op v1 (),env)])`
-             by metis_tac [e_step_add_ctxt, APPEND] >>
-     `e_step_reln (cenv,env''',Val v2,[(Capp2 op v1 (),env)])
-                  (cenv,env',Exp e'',[])`
-             by rw [e_step_def, e_step_reln_def, continue_def] >>
-     `e_step_reln^* (cenv,env,Exp e,[(Capp1 op () e',env)])
-                  (cenv,env',Exp e'',[])`
+     `e_step_reln (cenv,s2,env',Val v,[(Cuapp uop (),env)])
+                  (cenv,s3,env,Val v',[])`
+             by rw [e_step_def, e_step_reln_def, continue_def, return_def] >>
+     `e_step_reln^* (cenv,s,env,Exp e,[(Cuapp uop (),env)])
+                    (cenv,s3,env,Val v',[])`
               by metis_tac [transitive_RTC, RTC_SINGLE, transitive_def] >>
      metis_tac [small_eval_prefix],
  fs [small_eval_def] >>
-     `e_step_reln^* (cenv,env,Exp e,[(Capp1 op () e',env)])
-                (cenv,env',Val v1,[(Capp1 op () e',env)])`
+     `e_step_reln^* (cenv,s,env,Exp e,[(Cuapp uop (),env)])
+                    (cenv,s2,env',Val v,[(Cuapp uop (),env)])`
              by metis_tac [e_step_add_ctxt, APPEND] >>
-     `e_step_reln (cenv,env',Val v1,[(Capp1 op () e',env)])
-                  (cenv,env,Exp e',[(Capp2 op v1 (),env)])`
+     `e_step (cenv,s2,env',Val v,[(Cuapp uop (),env)]) = Etype_error`
              by rw [e_step_def, e_step_reln_def, continue_def, push_def] >>
-     `e_step_reln^* (cenv,env,Exp e',[(Capp2 op v1 (),env)])
-                    (cenv,env'',Val v2,[(Capp2 op v1 (),env)])`
+     metis_tac [transitive_RTC, RTC_SINGLE, transitive_def],
+ metis_tac [small_eval_err_add_ctxt, APPEND],
+ fs [small_eval_def] >>
+     `e_step_reln^* (cenv,s,env,Exp e,[(Capp1 op () e',env)])
+                    (cenv,s',env'',Val v1,[(Capp1 op () e',env)])`
              by metis_tac [e_step_add_ctxt, APPEND] >>
-     `e_step (cenv,env'',Val v2,[(Capp2 op v1 (),env)]) = Etype_error`
+     `e_step_reln (cenv,s',env'',Val v1,[(Capp1 op () e',env)])
+                  (cenv,s',env,Exp e',[(Capp2 op v1 (),env)])`
+             by rw [e_step_def, e_step_reln_def, continue_def, push_def] >>
+     `e_step_reln^* (cenv,s',env,Exp e',[(Capp2 op v1 (),env)])
+                    (cenv,s3,env''',Val v2,[(Capp2 op v1 (),env)])`
+             by metis_tac [e_step_add_ctxt, APPEND] >>
+     `e_step_reln (cenv,s3,env''',Val v2,[(Capp2 op v1 (),env)])
+                  (cenv,s'',env',Exp e'',[])`
+             by rw [e_step_def, e_step_reln_def, continue_def] >>
+     `e_step_reln^* (cenv,s,env,Exp e,[(Capp1 op () e',env)])
+                    (cenv,s'',env',Exp e'',[])`
+              by metis_tac [transitive_RTC, RTC_SINGLE, transitive_def] >>
+     metis_tac [small_eval_prefix],
+ fs [small_eval_def] >>
+     `e_step_reln^* (cenv,s,env,Exp e,[(Capp1 op () e',env)])
+                    (cenv,s',env',Val v1,[(Capp1 op () e',env)])`
+             by metis_tac [e_step_add_ctxt, APPEND] >>
+     `e_step_reln (cenv,s',env',Val v1,[(Capp1 op () e',env)])
+                  (cenv,s',env,Exp e',[(Capp2 op v1 (),env)])`
+             by rw [e_step_def, e_step_reln_def, continue_def, push_def] >>
+     `e_step_reln^* (cenv,s',env,Exp e',[(Capp2 op v1 (),env)])
+                    (cenv,s3,env'',Val v2,[(Capp2 op v1 (),env)])`
+             by metis_tac [e_step_add_ctxt, APPEND] >>
+     `e_step (cenv,s3,env'',Val v2,[(Capp2 op v1 (),env)]) = Etype_error`
              by rw [e_step_def, e_step_reln_def, continue_def, push_def] >>
      metis_tac [transitive_RTC, RTC_SINGLE, transitive_def],
  fs [small_eval_def] >>
-     `e_step_reln^* (cenv,env,Exp e,[(Capp1 op () e',env)])
-                (cenv,env',Val v1,[(Capp1 op () e',env)])`
+     `e_step_reln^* (cenv,s,env,Exp e,[(Capp1 op () e',env)])
+                    (cenv,s',env',Val v1,[(Capp1 op () e',env)])`
              by metis_tac [e_step_add_ctxt, APPEND] >>
-     `e_step_reln (cenv,env',Val v1,[(Capp1 op () e',env)])
-                  (cenv,env,Exp e',[(Capp2 op v1 (),env)])`
+     `e_step_reln (cenv,s',env',Val v1,[(Capp1 op () e',env)])
+                  (cenv,s',env,Exp e',[(Capp2 op v1 (),env)])`
              by rw [e_step_def, e_step_reln_def, continue_def, push_def] >>
-     `small_eval cenv env e' [(Capp2 op v1 (),env)] (Rerr err)`
+     `small_eval cenv s' env e' [(Capp2 op v1 (),env)] (Rerr err)`
              by metis_tac [small_eval_err_add_ctxt, APPEND] >>
-     `e_step_reln^* (cenv,env,Exp e,[(Capp1 op () e',env)])
-                    (cenv,env,Exp e',[(Capp2 op v1 (),env)])`
+     `e_step_reln^* (cenv,s,env,Exp e,[(Capp1 op () e',env)])
+                    (cenv,s',env,Exp e',[(Capp2 op v1 (),env)])`
              by metis_tac [transitive_RTC, RTC_SINGLE, transitive_def] >>
      metis_tac [small_eval_prefix],
  metis_tac [small_eval_err_add_ctxt, APPEND],
  fs [small_eval_def] >>
-     `e_step_reln^* (cenv,env,Exp e,[(Clog op () e2,env)])
-                (cenv,env',Val v,[(Clog op () e2,env)])`
+     `e_step_reln^* (cenv,s,env,Exp e,[(Clog op () e2,env)])
+                    (cenv,s',env',Val v,[(Clog op () e2,env)])`
              by metis_tac [e_step_add_ctxt, APPEND] >>
-     `e_step_reln (cenv,env',Val v,[(Clog op () e2,env)])
-                  (cenv,env,Exp e',[])`
+     `e_step_reln (cenv,s',env',Val v,[(Clog op () e2,env)])
+                  (cenv,s',env,Exp e',[])`
              by rw [e_step_def, e_step_reln_def, continue_def, push_def] >>
-     metis_tac [transitive_RTC, RTC_SINGLE, transitive_def,
-                small_eval_prefix],
+     metis_tac [transitive_RTC, RTC_SINGLE, transitive_def, small_eval_prefix],
  fs [small_eval_def] >>
-     `e_step_reln^* (cenv,env,Exp e,[(Clog op () e2,env)])
-                (cenv,env',Val v,[(Clog op () e2,env)])`
+     `e_step_reln^* (cenv,s,env,Exp e,[(Clog op () e2,env)])
+                    (cenv,s2,env',Val v,[(Clog op () e2,env)])`
              by metis_tac [e_step_add_ctxt, APPEND] >>
-     `e_step (cenv,env',Val v,[(Clog op () e2,env)]) = Etype_error`
+     `e_step (cenv,s2,env',Val v,[(Clog op () e2,env)]) = Etype_error`
              by rw [e_step_def, e_step_reln_def, continue_def, push_def] >>
      metis_tac [transitive_RTC, RTC_SINGLE, transitive_def],
  metis_tac [small_eval_err_add_ctxt, APPEND],
  fs [small_eval_def] >>
-     `e_step_reln^* (cenv,env,Exp e,[(Cif () e2 e3,env)])
-                (cenv,env',Val v,[(Cif () e2 e3,env)])`
+     `e_step_reln^* (cenv,s,env,Exp e,[(Cif () e2 e3,env)])
+                    (cenv,s',env',Val v,[(Cif () e2 e3,env)])`
              by metis_tac [e_step_add_ctxt, APPEND] >>
-     `e_step_reln (cenv,env',Val v,[(Cif () e2 e3,env)])
-                  (cenv,env,Exp e',[])`
+     `e_step_reln (cenv,s',env',Val v,[(Cif () e2 e3,env)])
+                  (cenv,s',env,Exp e',[])`
              by rw [e_step_def, e_step_reln_def, continue_def, push_def] >>
      metis_tac [transitive_RTC, RTC_SINGLE, transitive_def,
                 small_eval_prefix],
  fs [small_eval_def] >>
-     `e_step_reln^* (cenv,env,Exp e,[(Cif () e2 e3,env)])
-                (cenv,env',Val v,[(Cif () e2 e3,env)])`
+     `e_step_reln^* (cenv,s,env,Exp e,[(Cif () e2 e3,env)])
+                    (cenv,s2,env',Val v,[(Cif () e2 e3,env)])`
              by metis_tac [e_step_add_ctxt, APPEND] >>
-     `e_step (cenv,env',Val v,[(Cif () e2 e3,env)]) = Etype_error`
+     `e_step (cenv,s2,env',Val v,[(Cif () e2 e3,env)]) = Etype_error`
              by rw [e_step_def, e_step_reln_def, continue_def, push_def] >>
      metis_tac [transitive_RTC, RTC_SINGLE, transitive_def],
  metis_tac [small_eval_err_add_ctxt, APPEND],
  fs [small_eval_def] >>
      imp_res_tac small_eval_match_thm >>
-     cases_on `r` >>
-     TRY (Cases_on `e'`) >>
+     cases_on `r` >|
+     [cases_on `a`,
+      cases_on `e'`] >>
      rw [] >>
      fs [small_eval_def, alt_small_eval_def] >>
      metis_tac [transitive_def, transitive_RTC, e_step_add_ctxt, APPEND],
  metis_tac [small_eval_err_add_ctxt, APPEND],
  fs [small_eval_def] >>
-     `e_step_reln^* (cenv,env,Exp e,[(Clet n () e',env)])
-                (cenv,env',Val v,[(Clet n () e',env)])`
+     `e_step_reln^* (cenv,s,env,Exp e,[(Clet n () e',env)])
+                    (cenv,s',env',Val v,[(Clet n () e',env)])`
              by metis_tac [e_step_add_ctxt, APPEND] >>
-     `e_step_reln (cenv,env',Val v,[(Clet n () e',env)])
-                  (cenv,bind n v env,Exp e',[])`
+     `e_step_reln (cenv,s',env',Val v,[(Clet n () e',env)])
+                  (cenv,s',bind n v env,Exp e',[])`
              by rw [e_step_def, e_step_reln_def, continue_def, push_def] >>
      metis_tac [transitive_RTC, RTC_SINGLE, transitive_def,
                 small_eval_prefix],
  metis_tac [small_eval_err_add_ctxt, APPEND],
  rw [small_eval_def] >>
+     qexists_tac `s` >>
      qexists_tac `env` >>
      qexists_tac `Exp (Letrec funs e)` >>
      qexists_tac `[]` >>
@@ -605,16 +641,16 @@ rw [small_eval_app, small_eval_log, small_eval_if, small_eval_match,
  metis_tac [small_eval_match_rules]]);
 
 val evaluate_ctxts_cons = Q.prove (
-`!cenv f cs v bv.
-  evaluate_ctxts cenv (f::cs) v bv =
-  (?c env v'.
+`!cenv s1 f cs v bv.
+  evaluate_ctxts cenv s1 (f::cs) v bv =
+  (?c s2 env v'.
      (f = (c,env)) ∧
-     evaluate_ctxt cenv env c v (Rval v') ∧
-     evaluate_ctxts cenv cs v' bv) ∨
+     evaluate_ctxt cenv s1 env c v (Rval (s2,v')) ∧
+     evaluate_ctxts cenv s2 cs v' bv) ∨
   (?c env err.
      (f = (c,env)) ∧
      (bv = Rerr err) ∧
-     evaluate_ctxt cenv env c v (Rerr err))`,
+     evaluate_ctxt cenv s1 env c v (Rerr err))`,
 rw [] >>
 rw [Once evaluate_ctxts_cases] >>
 EQ_TAC >>
@@ -622,23 +658,78 @@ rw [] >>
 metis_tac []);
 
 val evaluate_raise = Q.prove (
-`!cenv env err bv.
-  (evaluate cenv env (Raise err) bv = (bv = Rerr (Rraise err)))`,
+`!cenv s env err bv.
+  (evaluate cenv s env (Raise err) bv = (bv = Rerr (Rraise err)))`,
 rw [Once evaluate_cases]);
 
 val one_step_backward = Q.prove (
-`!cenv env e c cenv' env' e' c' bv.
-  (e_step (cenv,env,e,c) = Estep (cenv',env',e',c')) ∧
-  evaluate_state (cenv',env',e',c') bv
+`!cenv s env e c cenv' s' env' e' c' bv.
+  (e_step (cenv,s,env,e,c) = Estep (cenv',s',env',e',c')) ∧
+  evaluate_state (cenv',s',env',e',c') bv
   ⇒
-  evaluate_state (cenv,env,e,c) bv`,
+  evaluate_state (cenv,s,env,e,c) bv`,
 rw [e_step_def] >>
 cases_on `e` >>
 fs [] >>
 every_case_tac >>
 fs [push_def,return_def] >>
 rw [] >|
-[fs [evaluate_state_cases, Once evaluate_cases],
+[fs [evaluate_state_cases, Once evaluate_cases] >>
+     metis_tac [],
+ fs [evaluate_state_cases] >>
+     ONCE_REWRITE_TAC [evaluate_cases] >>
+     ONCE_REWRITE_TAC [hd (tl (CONJUNCTS evaluate_cases))] >>
+     rw [] >>
+     fs [evaluate_ctxts_cons, evaluate_ctxt_cases] >>
+     metis_tac [],
+ fs [evaluate_state_cases] >>
+     ONCE_REWRITE_TAC [evaluate_cases] >>
+     ONCE_REWRITE_TAC [hd (tl (CONJUNCTS evaluate_cases))] >>
+     rw [] >>
+     fs [evaluate_ctxts_cons, evaluate_ctxt_cases, arithmeticTheory.ADD1] >>
+     rw [] >>
+     metis_tac [],
+ fs [evaluate_state_cases, Once evaluate_cases] >>
+     metis_tac [],
+ fs [evaluate_state_cases, Once evaluate_cases] >>
+     metis_tac [],
+ fs [evaluate_state_cases, Once evaluate_ctxts_cases] >>
+     ONCE_REWRITE_TAC [evaluate_cases] >>
+     rw [] >>
+     fs [evaluate_ctxt_cases, Once evaluate_ctxts_cases] >>
+     metis_tac [],
+ fs [evaluate_state_cases, Once evaluate_ctxts_cases] >>
+     ONCE_REWRITE_TAC [evaluate_cases] >>
+     rw [] >>
+     fs [evaluate_ctxt_cases, Once evaluate_ctxts_cases] >>
+     metis_tac [],
+ fs [evaluate_state_cases, Once evaluate_ctxts_cases] >>
+     ONCE_REWRITE_TAC [evaluate_cases] >>
+     rw [] >>
+     fs [evaluate_ctxt_cases, Once evaluate_ctxts_cases] >>
+     metis_tac [],
+ fs [evaluate_state_cases, Once evaluate_ctxts_cases] >>
+     ONCE_REWRITE_TAC [evaluate_cases] >>
+     rw [] >>
+     fs [evaluate_ctxt_cases, Once evaluate_ctxts_cases] >>
+     metis_tac [],
+ fs [evaluate_state_cases, Once evaluate_ctxts_cases] >>
+     ONCE_REWRITE_TAC [evaluate_cases] >>
+     rw [] >>
+     fs [evaluate_ctxt_cases, Once evaluate_ctxts_cases] >>
+     metis_tac [],
+ fs [evaluate_state_cases, Once evaluate_ctxts_cases] >>
+     ONCE_REWRITE_TAC [evaluate_cases] >>
+     rw [] >>
+     fs [evaluate_ctxt_cases, Once evaluate_ctxts_cases] >>
+     metis_tac [],
+ fs [evaluate_state_cases, Once evaluate_ctxts_cases] >>
+     ONCE_REWRITE_TAC [evaluate_cases] >>
+     rw [] >>
+     fs [evaluate_ctxt_cases, Once evaluate_ctxts_cases] >>
+     metis_tac [],
+ fs [evaluate_state_cases, Once evaluate_cases],
+ fs [evaluate_state_cases, Once evaluate_cases],
  fs [evaluate_state_cases] >>
      ONCE_REWRITE_TAC [evaluate_cases] >>
      ONCE_REWRITE_TAC [hd (tl (CONJUNCTS evaluate_cases))] >>
@@ -653,52 +744,12 @@ rw [] >|
      metis_tac [],
  fs [evaluate_state_cases, Once evaluate_cases],
  fs [evaluate_state_cases, Once evaluate_cases],
- fs [evaluate_state_cases, Once evaluate_ctxts_cases] >>
-     ONCE_REWRITE_TAC [evaluate_cases] >>
-     rw [] >>
-     fs [evaluate_ctxt_cases, Once evaluate_ctxts_cases] >>
-     metis_tac [],
- fs [evaluate_state_cases, Once evaluate_ctxts_cases] >>
-     ONCE_REWRITE_TAC [evaluate_cases] >>
-     rw [] >>
-     fs [evaluate_ctxt_cases, Once evaluate_ctxts_cases] >>
-     metis_tac [],
- fs [evaluate_state_cases, Once evaluate_ctxts_cases] >>
-     ONCE_REWRITE_TAC [evaluate_cases] >>
-     rw [] >>
-     fs [evaluate_ctxt_cases, Once evaluate_ctxts_cases] >>
-     metis_tac [],
- fs [evaluate_state_cases, Once evaluate_ctxts_cases] >>
-     ONCE_REWRITE_TAC [evaluate_cases] >>
-     rw [] >>
-     fs [evaluate_ctxt_cases, Once evaluate_ctxts_cases] >>
-     metis_tac [],
- fs [evaluate_state_cases, Once evaluate_ctxts_cases] >>
-     ONCE_REWRITE_TAC [evaluate_cases] >>
-     rw [] >>
-     fs [evaluate_ctxt_cases, Once evaluate_ctxts_cases] >>
-     metis_tac [],
- fs [evaluate_state_cases, Once evaluate_ctxts_cases] >>
-     ONCE_REWRITE_TAC [evaluate_cases] >>
-     rw [] >>
-     fs [evaluate_ctxt_cases, Once evaluate_ctxts_cases] >>
-     metis_tac [],
- fs [evaluate_state_cases, Once evaluate_cases],
- fs [evaluate_state_cases, Once evaluate_cases],
  fs [evaluate_state_cases] >>
      ONCE_REWRITE_TAC [evaluate_cases] >>
-     ONCE_REWRITE_TAC [hd (tl (CONJUNCTS evaluate_cases))] >>
      rw [] >>
-     fs [evaluate_ctxts_cons, evaluate_ctxt_cases],
- fs [evaluate_state_cases] >>
-     ONCE_REWRITE_TAC [evaluate_cases] >>
-     ONCE_REWRITE_TAC [hd (tl (CONJUNCTS evaluate_cases))] >>
-     rw [] >>
-     fs [evaluate_ctxts_cons, evaluate_ctxt_cases, arithmeticTheory.ADD1] >>
+     fs [evaluate_ctxts_cons, evaluate_ctxt_cases] >>
      rw [] >>
      metis_tac [],
- fs [evaluate_state_cases, Once evaluate_cases],
- fs [evaluate_state_cases, Once evaluate_cases],
  fs [evaluate_state_cases] >>
      ONCE_REWRITE_TAC [evaluate_cases] >>
      rw [] >>
@@ -797,10 +848,10 @@ rw [] >|
           metis_tac [APPEND_ASSOC, APPEND]]]);
 
 val one_step_backward_type_error = Q.prove (
-`!cenv env e c.
-  (e_step (cenv,env,e,c) = Etype_error)
+`!cenv s env e c.
+  (e_step (cenv,s,env,e,c) = Etype_error)
   ⇒
-  evaluate_state (cenv,env,e,c) (Rerr Rtype_error)`,
+  evaluate_state (cenv,s,env,e,c) (Rerr Rtype_error)`,
 rw [e_step_def] >>
 cases_on `e` >>
 fs [] >>
@@ -846,43 +897,31 @@ val small_exp_to_big_exp = Q.prove (
     evaluate_state st r`,
 HO_MATCH_MP_TAC RTC_INDUCT_RIGHT1 >>
 rw [e_step_reln_def] >>
-`?cenv env e c. st = (cenv, env, e, c)`
-        by (cases_on `st` >>
-            cases_on `r'` >>
-            cases_on `r''` >>
-            rw []) >>
-rw [] >>
-`?cenv' env' e' c'. st' = (cenv', env', e', c')`
-        by (cases_on `st'` >>
-            cases_on `r'` >>
-            cases_on `r''` >>
-            rw []) >>
-rw [] >>
-`?cenv'' env'' e'' c''. st'' = (cenv'', env'', e'', c'')`
-        by (cases_on `st''` >>
-            cases_on `r'` >>
-            cases_on `r''` >>
-            rw []) >>
+PairCases_on `st` >>
+PairCases_on `st'` >>
+PairCases_on `st''` >>
 rw [] >>
 metis_tac [one_step_backward]);
 
 val evaluate_state_no_ctxt = Q.prove (
-`!envc env e r. evaluate_state (envc,env,Exp e,[]) r = evaluate envc env e r`,
+`!envc s env e r. evaluate_state (envc,s,env,Exp e,[]) r = evaluate envc s env e r`,
 rw [evaluate_state_cases, Once evaluate_ctxts_cases] >>
-cases_on `r` >>
+cases_on `r` >|
+[cases_on `a`,
+ cases_on `e'`] >>
 rw [] >>
 metis_tac []);
 
 val evaluate_state_val_no_ctxt = Q.prove (
-`!envc env e. evaluate_state (envc,env,Val e,[]) r = (r = Rval e)`,
+`!envc s env e. evaluate_state (envc,s,env,Val e,[]) r = (r = Rval (s,e))`,
 rw [evaluate_state_cases, Once evaluate_ctxts_cases] >>
 rw [evaluate_state_cases, Once evaluate_ctxts_cases]);
 
 val small_big_exp_equiv = Q.store_thm ("small_big_exp_equiv",
-`!envc env e r. small_eval envc env e [] r = evaluate envc env e r`,
+`!envc s env e r. small_eval envc s env e [] r = evaluate envc s env e r`,
 rw [] >>
 cases_on `r` >|
-[all_tac,
+[cases_on `a`,
  cases_on `e'`] >>
 rw [small_eval_def] >>
 EQ_TAC >>
@@ -892,11 +931,11 @@ metis_tac [small_exp_to_big_exp, big_exp_to_small_exp,
            one_step_backward_type_error, evaluate_state_val_no_ctxt]);
 
 val lift_small_exp_to_dec_one_step = Q.prove (
-`!cenv env e c cenv' env' e' c' cenv'' env'' ds p.
-  e_step_reln (cenv,env,e,c) (cenv',env',e',c')
+`!cenv s env e c cenv' s' env' e' c' cenv'' s'' env'' ds p.
+  e_step_reln (cenv,s,env,e,c) (cenv',s',env',e',c')
   ⇒
-  d_step_reln (cenv'',env'',ds,SOME (p,(cenv,env,e,c)))
-              (cenv'',env'',ds,SOME (p,(cenv',env',e',c')))`,
+  d_step_reln (cenv'',s'',env'',ds,SOME (p,(cenv,s,env,e,c)))
+              (cenv'',empty_store,env'',ds,SOME (p,(cenv',s',env',e',c')))`,
 rw [e_step_reln_def, d_step_reln_def, d_step_def] >>
 every_case_tac >>
 fs [e_step_def, continue_def, push_def, return_def] >>
@@ -905,89 +944,82 @@ rw []);
 val lift_small_exp_to_dec = Q.prove (
 `!st st'. e_step_reln^* st st' ⇒
    !p cenv'' env'' ds.
-     d_step_reln^* (cenv'',env'',ds,SOME (p,st)) (cenv'',env'',ds,SOME (p,st'))`,
+     d_step_reln^* (cenv'',empty_store,env'',ds,SOME (p,st)) (cenv'',empty_store,env'',ds,SOME (p,st'))`,
 HO_MATCH_MP_TAC RTC_INDUCT >>
 rw [] >>
-`?cenv env e c. st = (cenv, env, e, c)`
-        by (cases_on `st` >>
-            cases_on `r` >>
-            cases_on `r'` >>
-            rw []) >>
-rw [] >>
-`?cenv' env' e' c'. st' = (cenv', env', e', c')`
-        by (cases_on `st'` >>
-            cases_on `r` >>
-            cases_on `r'` >>
-            rw []) >>
+PairCases_on `st` >>
+PairCases_on `st'` >>
+PairCases_on `st''` >>
 rw [] >>
 metis_tac [lift_small_exp_to_dec_one_step, transitive_def, transitive_RTC,
            RTC_SINGLE]);
 
 val big_dec_to_small_dec = Q.prove (
-`!cenv env ds r.
-  evaluate_decs cenv env ds r ⇒ d_small_eval cenv env ds NONE r`,
+`!cenv s env ds r.
+  evaluate_decs cenv s env ds r ⇒ d_small_eval cenv s env ds NONE r`,
 HO_MATCH_MP_TAC evaluate_decs_ind >>
 rw [d_small_eval_def] >|
-[cases_on `r` >>
-     TRY (cases_on `a`) >>
-     fs [d_small_eval_def] >|
-     [`d_step_reln (cenv,env,Dlet p e::ds,NONE)
-                   (cenv,env,ds,SOME(p,cenv,env,Exp e,[]))`
+[cases_on `r` >|
+     [`?cenv2 s2 env2. a = (cenv2,s2,env2)`
+                by (PairCases_on `a` >> rw []) >>
+          fs [d_small_eval_def] >>
+          `d_step_reln (cenv,s,env,Dlet p e::ds,NONE)
+                       (cenv,empty_store,env,ds,SOME(p,cenv,s,env,Exp e,[]))`
                 by (rw [d_step_reln_def, d_step_def]) >>
           imp_res_tac big_exp_to_small_exp >>
           fs [small_eval_def] >>
-          `d_step_reln^* (cenv,env,ds,SOME (p,(cenv,env,Exp e,[])))
-                         (cenv,env,ds,SOME (p,(cenv,env'',Val v,[])))`
+          `d_step_reln^* (cenv,empty_store,env,ds,SOME (p,(cenv,s,env,Exp e,[])))
+                         (cenv,empty_store,env,ds,SOME (p,(cenv,s',env'',Val v,[])))`
                        by metis_tac [lift_small_exp_to_dec] >>
-          `d_step_reln (cenv,env,ds,SOME (p,(cenv,env'',Val v,[])))
-                         (cenv,env',ds,NONE)`
+          `d_step_reln (cenv,empty_store,env,ds,SOME (p,(cenv,s',env'',Val v,[])))
+                       (cenv,s',env',ds,NONE)`
                 by rw [d_step_reln_def, d_step_def] >>
           metis_tac [RTC_SINGLE, transitive_RTC, transitive_def],
       cases_on `e'` >>
           fs [d_small_eval_def] >>
-          `d_step_reln (cenv,env,Dlet p e::ds,NONE)
-                   (cenv,env,ds,SOME(p,cenv,env,Exp e,[]))`
+          `d_step_reln (cenv,s,env,Dlet p e::ds,NONE)
+                       (cenv,empty_store,env,ds,SOME(p,cenv,s,env,Exp e,[]))`
                 by (rw [d_step_reln_def, d_step_def]) >>
           imp_res_tac big_exp_to_small_exp >>
           fs [small_eval_def] >>
-          `d_step_reln^* (cenv,env,ds,SOME (p,(cenv,env,Exp e,[])))
-                         (cenv,env,ds,SOME (p,(cenv,env''',Val v,[])))`
+          `d_step_reln^* (cenv,empty_store,env,ds,SOME (p,(cenv,s,env,Exp e,[])))
+                         (cenv,empty_store,env,ds,SOME (p,(cenv,s',env''',Val v,[])))`
                        by metis_tac [lift_small_exp_to_dec] >>
-          `d_step_reln (cenv,env,ds,SOME (p,(cenv,env''',Val v,[])))
-                         (cenv,env',ds,NONE)`
+          `d_step_reln (cenv,empty_store,env,ds,SOME (p,(cenv,s',env''',Val v,[])))
+                       (cenv,s',env',ds,NONE)`
                 by rw [d_step_reln_def, d_step_def] >>
           metis_tac [RTC_SINGLE, transitive_RTC, transitive_def]],
- `d_step_reln (cenv,env,Dlet p e::ds,NONE)
-                   (cenv,env,ds,SOME(p,cenv,env,Exp e,[]))`
+ `d_step_reln (cenv,s,env,Dlet p e::ds,NONE)
+              (cenv,empty_store,env,ds,SOME(p,cenv,s,env,Exp e,[]))`
                 by (rw [d_step_reln_def, d_step_def]) >>
      imp_res_tac big_exp_to_small_exp >>
      fs [small_eval_def] >>
-     `d_step_reln^* (cenv,env,ds,SOME (p,(cenv,env,Exp e,[])))
-                    (cenv,env,ds,SOME (p,(cenv,env',Val v,[])))`
+     `d_step_reln^* (cenv,empty_store,env,ds,SOME (p,(cenv,s,env,Exp e,[])))
+                    (cenv,empty_store,env,ds,SOME (p,(cenv,s2,env',Val v,[])))`
                   by metis_tac [lift_small_exp_to_dec] >>
-     `d_step (cenv,env,ds,SOME (p,(cenv,env',Val v,[]))) = Draise Bind_error`
+     `d_step (cenv,empty_store,env,ds,SOME (p,(cenv,s2,env',Val v,[]))) = Draise Bind_error`
                by rw [d_step_reln_def, d_step_def] >>
      metis_tac [RTC_SINGLE, transitive_RTC, transitive_def],
- `d_step_reln (cenv,env,Dlet p e::ds,NONE)
-                   (cenv,env,ds,SOME(p,cenv,env,Exp e,[]))`
+ `d_step_reln (cenv,s,env,Dlet p e::ds,NONE)
+              (cenv,empty_store,env,ds,SOME(p,cenv,s,env,Exp e,[]))`
                 by (rw [d_step_reln_def, d_step_def]) >>
      imp_res_tac big_exp_to_small_exp >>
      fs [small_eval_def] >>
-     `d_step_reln^* (cenv,env,ds,SOME (p,(cenv,env,Exp e,[])))
-                    (cenv,env,ds,SOME (p,(cenv,env',Val v,[])))`
+     `d_step_reln^* (cenv,empty_store,env,ds,SOME (p,(cenv,s,env,Exp e,[])))
+                    (cenv,empty_store,env,ds,SOME (p,(cenv,s2,env',Val v,[])))`
                   by metis_tac [lift_small_exp_to_dec] >>
-     `d_step (cenv,env,ds,SOME (p,(cenv,env',Val v,[]))) = Dtype_error`
+     `d_step (cenv,empty_store,env,ds,SOME (p,(cenv,s2,env',Val v,[]))) = Dtype_error`
                by rw [d_step_reln_def, d_step_def] >>
      metis_tac [RTC_SINGLE, transitive_RTC, transitive_def],
- `d_step_reln (cenv,env,Dlet p e::ds,NONE)
-              (cenv,env,ds,SOME(p,cenv,env,Exp e,[]))`
+ `d_step_reln (cenv,s,env,Dlet p e::ds,NONE)
+              (cenv,empty_store,env,ds,SOME(p,cenv,s,env,Exp e,[]))`
                 by (rw [d_step_reln_def, d_step_def]) >>
      imp_res_tac big_exp_to_small_exp >>
      fs [small_eval_def] >>
-     `d_step_reln^* (cenv,env,ds,SOME (p,(cenv,env,Exp e,[])))
-                    (cenv,env,ds,SOME (p,(cenv,env',Val v,[])))`
+     `d_step_reln^* (cenv,empty_store,env,ds,SOME (p,(cenv,s,env,Exp e,[])))
+                    (cenv,empty_store,env,ds,SOME (p,(cenv,s2,env',Val v,[])))`
                    by metis_tac [lift_small_exp_to_dec] >>
-     `d_step (cenv,env,ds,SOME (p,(cenv,env',Val v,[]))) = Dtype_error`
+     `d_step (cenv,empty_store,env,ds,SOME (p,(cenv,s2,env',Val v,[]))) = Dtype_error`
                  by (rw [d_step_def] >>
                      every_case_tac >>
                      fs [] >>
@@ -995,93 +1027,95 @@ rw [d_small_eval_def] >|
      metis_tac [RTC_SINGLE, transitive_RTC, transitive_def],
  cases_on `err` >>
      fs [d_small_eval_def] >>
-     `d_step_reln (cenv,env,Dlet p e::ds,NONE)
-                   (cenv,env,ds,SOME(p,cenv,env,Exp e,[]))`
+     `d_step_reln (cenv,s,env,Dlet p e::ds,NONE)
+                  (cenv,empty_store,env,ds,SOME(p,cenv,s,env,Exp e,[]))`
                 by (rw [d_step_reln_def, d_step_def]) >>
      imp_res_tac big_exp_to_small_exp >>
      fs [small_eval_def] >|
-     [`d_step_reln^* (cenv,env,ds,SOME (p,(cenv,env,Exp e,[])))
-                     (cenv,env,ds,SOME (p,(cenv,env', e',c')))`
+     [`d_step_reln^* (cenv,empty_store,env,ds,SOME (p,(cenv,s,env,Exp e,[])))
+                     (cenv,empty_store,env,ds,SOME (p,(cenv,s',env', e',c')))`
                    by metis_tac [lift_small_exp_to_dec] >>
-          `d_step (cenv,env,ds,SOME (p,(cenv,env', e',c'))) = Dtype_error`
+          `d_step (cenv,empty_store,env,ds,SOME (p,(cenv,s',env', e',c'))) = Dtype_error`
                  by (rw [d_step_def] >>
                      every_case_tac >>
                      fs [] >>
                      fs [e_step_def, continue_def]) >>
           metis_tac [RTC_SINGLE, transitive_RTC, transitive_def],
-      `d_step_reln^* (cenv,env,ds,SOME (p,(cenv,env,Exp e,[])))
-                     (cenv,env,ds,SOME (p,(cenv,env',Exp (Raise e'),[])))`
+      `d_step_reln^* (cenv,empty_store,env,ds,SOME (p,(cenv,s,env,Exp e,[])))
+                     (cenv,empty_store,env,ds,SOME (p,(cenv,s',env',Exp (Raise e'),[])))`
                    by metis_tac [lift_small_exp_to_dec] >>
-          `d_step (cenv,env,ds,SOME (p,(cenv,env',Exp (Raise e'),[]))) = Draise e'`
+          `d_step (cenv,empty_store,env,ds,SOME (p,(cenv,s',env',Exp (Raise e'),[]))) = Draise e'`
                  by (rw [d_step_def] >>
                      every_case_tac >>
                      fs [] >>
                      fs [e_step_def, continue_def]) >>
           metis_tac [RTC_SINGLE, transitive_RTC, transitive_def]],
  cases_on `r` >|
-     [cases_on `a`,
+     [`?cenv2 s2 env2. a = (cenv2,s2,env2)`
+                by (PairCases_on `a` >> rw []),
       cases_on `e`] >>
      fs [d_small_eval_def] >>
-     `d_step_reln (cenv,env,Dletrec funs::ds,NONE)
-                  (cenv,build_rec_env funs env, ds, NONE)`
+     `d_step_reln (cenv,s,env,Dletrec funs::ds,NONE)
+                  (cenv,s,build_rec_env funs env, ds, NONE)`
                by rw [d_step_reln_def, d_step_def] >>
      metis_tac [RTC_SINGLE, transitive_RTC, transitive_def],
- `d_step (cenv,env,Dletrec funs::ds,NONE) = Dtype_error`
+ `d_step (cenv,s,env,Dletrec funs::ds,NONE) = Dtype_error`
         by rw [d_step_def] >>
      metis_tac [RTC_REFL, transitive_RTC, transitive_def],
  cases_on `r` >|
-     [cases_on `a`,
+     [`?cenv2 s2 env2. a = (cenv2,s2,env2)`
+                by (PairCases_on `a` >> rw []),
       cases_on `e`] >>
      fs [d_small_eval_def] >>
-     `d_step_reln (cenv,env,Dtype tds::ds,NONE)
-                  (build_tdefs tds ++ cenv,env,ds,NONE)`
+     `d_step_reln (cenv,s,env,Dtype tds::ds,NONE)
+                  (build_tdefs tds ++ cenv,s,env,ds,NONE)`
                by rw [d_step_reln_def, d_step_def] >>
      metis_tac [merge_def,RTC_SINGLE, transitive_RTC, transitive_def],
- `d_step (cenv,env,Dtype tds::ds,NONE) = Dtype_error`
+ `d_step (cenv,s,env,Dtype tds::ds,NONE) = Dtype_error`
                by rw [d_step_def] >>
      metis_tac [RTC_REFL, transitive_RTC, transitive_def]]);
 
 val (evaluate_d_state_rules, evaluate_d_state_ind, evaluate_d_state_cases) = Hol_reln `
-(!cenv env ds r.
-   evaluate_decs cenv env ds r
+(!cenv s env ds r.
+   evaluate_decs cenv s env ds r
    ⇒
-   evaluate_d_state (cenv,env,ds,NONE) r) ∧
+   evaluate_d_state (cenv,s,env,ds,NONE) r) ∧
 
-(∀cenv env p e ds v env' r cenv' c env''.
-   evaluate_state (cenv',env',e,c) (Rval v) ∧ ALL_DISTINCT (pat_bindings p []) ∧
-   (pmatch cenv p v env = Match env'') ∧
-   evaluate_decs cenv env'' ds r ⇒
-   evaluate_d_state (cenv,env,ds,SOME (p,(cenv',env',e,c))) r) ∧
+(∀cenv s1 env p e ds v env' r cenv' s2 c env'' s_emp.
+   evaluate_state (cenv',s1,env',e,c) (Rval (s2,v)) ∧ ALL_DISTINCT (pat_bindings p []) ∧
+   (pmatch cenv s2 p v env = Match env'') ∧
+   evaluate_decs cenv s2 env'' ds r ⇒
+   evaluate_d_state (cenv,s_emp,env,ds,SOME (p,(cenv',s1,env',e,c))) r) ∧
 
-(∀cenv env p e ds v cenv' c env'.
-   evaluate_state (cenv',env',e,c) (Rval v) ∧ ALL_DISTINCT (pat_bindings p []) ∧
-   (pmatch cenv p v env = No_match) ⇒
-   evaluate_d_state (cenv,env,ds,SOME (p,(cenv',env',e,c))) (Rerr (Rraise Bind_error))) ∧
+(∀cenv s1 env p e ds v cenv' c s2 env' s_emp.
+   evaluate_state (cenv',s1,env',e,c) (Rval (s2,v)) ∧ ALL_DISTINCT (pat_bindings p []) ∧
+   (pmatch cenv s2 p v env = No_match) ⇒
+   evaluate_d_state (cenv,s_emp,env,ds,SOME (p,(cenv',s1,env',e,c))) (Rerr (Rraise Bind_error))) ∧
 
-(∀cenv env p e ds v cenv' c env'.
-   evaluate_state (cenv',env',e,c) (Rval v) ∧
-   (pmatch cenv p v env = Match_type_error) ⇒
-   evaluate_d_state (cenv,env,ds,SOME (p,(cenv',env',e,c))) (Rerr Rtype_error)) ∧
+(∀cenv s1 env p e ds v cenv' c s2 env' s_emp.
+   evaluate_state (cenv',s1,env',e,c) (Rval (s2,v)) ∧
+   (pmatch cenv s2 p v env = Match_type_error) ⇒
+   evaluate_d_state (cenv,s_emp,env,ds,SOME (p,(cenv',s1,env',e,c))) (Rerr Rtype_error)) ∧
 
-(∀cenv env p e ds v cenv' c env'.
-   evaluate_state (cenv',env',e,c) (Rval v) ∧ ¬ALL_DISTINCT (pat_bindings p []) ⇒
-   evaluate_d_state (cenv,env,ds,SOME (p,(cenv',env',e,c))) (Rerr Rtype_error)) ∧
+(∀cenv s1 env p e ds v cenv' c s2 env' s_emp.
+   evaluate_state (cenv',s1,env',e,c) (Rval (s2,v)) ∧ ¬ALL_DISTINCT (pat_bindings p []) ⇒
+   evaluate_d_state (cenv,s_emp,env,ds,SOME (p,(cenv',s1,env',e,c))) (Rerr Rtype_error)) ∧
 
-(∀cenv env p e ds err cenv' c env'.
-   evaluate_state (cenv',env',e,c)  (Rerr err) ⇒
-   evaluate_d_state (cenv,env,ds,SOME (p,(cenv',env',e,c))) (Rerr err)) ∧
+(∀cenv s env p e ds err cenv' c env' s_emp.
+   evaluate_state (cenv',s,env',e,c)  (Rerr err) ⇒
+   evaluate_d_state (cenv,s_emp,env,ds,SOME (p,(cenv',s,env',e,c))) (Rerr err)) ∧
 
-(!cenv env ds p cenv' env' e c err.
-  evaluate_state (cenv',env',e,c) (Rerr err)
+(!cenv s env ds p cenv' env' e c err s_emp.
+  evaluate_state (cenv',s,env',e,c) (Rerr err)
   ⇒
-  evaluate_d_state (cenv,env,ds,SOME (p,(cenv',env',e,c))) (Rerr err))`;
+  evaluate_d_state (cenv,s_emp,env,ds,SOME (p,(cenv',s,env',e,c))) (Rerr err))`;
 
 val one_step_backward_dec = Q.prove (
-`!cenv env ds c cenv' env' ds' c' r.
-  (d_step (cenv,env,ds,c) = Dstep (cenv',env',ds',c')) ∧
-  evaluate_d_state (cenv',env',ds',c') r
+`!cenv s env ds c cenv' s' env' ds' c' r.
+  (d_step (cenv,s,env,ds,c) = Dstep (cenv',s',env',ds',c')) ∧
+  evaluate_d_state (cenv',s',env',ds',c') r
   ⇒
-  evaluate_d_state (cenv,env,ds,c) r`,
+  evaluate_d_state (cenv,s,env,ds,c) r`,
 rw [d_step_def] >>
 cases_on `c` >>
 fs [] >>
@@ -1111,10 +1145,10 @@ rw [] >>
 metis_tac [one_step_backward, evaluate_state_val_no_ctxt]);
 
 val one_step_backward_dec_type_error = Q.prove (
-`!cenv env ds c.
-  (d_step (cenv,env,ds,c) = Dtype_error)
+`!cenv s env ds c.
+  (d_step (cenv,s,env,ds,c) = Dtype_error)
   ⇒
-  evaluate_d_state (cenv,env,ds,c) (Rerr Rtype_error)`,
+  evaluate_d_state (cenv,s,env,ds,c) (Rerr Rtype_error)`,
 rw [d_step_def] >>
 cases_on `c` >>
 fs [] >>
@@ -1126,10 +1160,10 @@ rw [Once evaluate_decs_cases] >>
 metis_tac [one_step_backward_type_error, evaluate_state_no_ctxt, evaluate_state_val_no_ctxt]);
 
 val one_step_backward_dec_error = Q.prove (
-`!cenv env ds c err.
-  (d_step (cenv,env,ds,c) = Draise err)
+`!cenv s env ds c err.
+  (d_step (cenv,s,env,ds,c) = Draise err)
   ⇒
-  evaluate_d_state (cenv,env,ds,c) (Rerr (Rraise err))`,
+  evaluate_d_state (cenv,s,env,ds,c) (Rerr (Rraise err))`,
 rw [d_step_def] >>
 cases_on `c` >>
 fs [] >>
@@ -1147,41 +1181,29 @@ val small_dec_to_big_dec = Q.prove (
     evaluate_d_state st r`,
 HO_MATCH_MP_TAC RTC_INDUCT_RIGHT1 >>
 rw [d_step_reln_def] >>
-`?cenv env ds c. st = (cenv, env, ds, c)`
-        by (cases_on `st` >>
-            cases_on `r'` >>
-            cases_on `r''` >>
-            rw []) >>
-rw [] >>
-`?cenv' env' ds' c'. st' = (cenv', env', ds', c')`
-        by (cases_on `st'` >>
-            cases_on `r'` >>
-            cases_on `r''` >>
-            rw []) >>
-rw [] >>
-`?cenv'' env'' ds'' c''. st'' = (cenv'', env'', ds'', c'')`
-        by (cases_on `st''` >>
-            cases_on `r'` >>
-            cases_on `r''` >>
-            rw []) >>
+PairCases_on `st` >>
+PairCases_on `st'` >>
+PairCases_on `st''` >>
 rw [] >>
 metis_tac [one_step_backward_dec]);
 
 val evaluate_d_state_no_ctxt = Q.prove (
-`!envc env ds r.
-  evaluate_d_state (envc,env,ds,NONE) r = evaluate_decs envc env ds r`,
+`!envc s env ds r.
+  evaluate_d_state (envc,s,env,ds,NONE) r = evaluate_decs envc s env ds r`,
 rw [evaluate_d_state_cases]);
 
 val evaluate_d_state_val = Q.prove (
-`!cenv env. evaluate_d_state (cenv,env,[],NONE) (Rval (cenv,env))`,
+`!cenv s env. evaluate_d_state (cenv,s,env,[],NONE) (Rval (cenv,s,env))`,
 rw [evaluate_d_state_cases] >>
 rw [Once evaluate_decs_cases]);
 
 val small_big_equiv = Q.store_thm ("small_big_equiv",
-`!envc env ds r. d_small_eval envc env ds NONE r = evaluate_decs envc env ds r`,
+`!envc s env ds r. d_small_eval envc s env ds NONE r = evaluate_decs envc s env ds r`,
 rw [] >>
 cases_on `r` >|
-[cases_on `a`,
+[`?cenv s env. a = (cenv,s,env)` 
+           by (PairCases_on `a` >>
+               rw[]  ),
  cases_on `e`] >>
 rw [d_small_eval_def] >>
 EQ_TAC >>
